\section{Differentiation}

\subsection*{Common Differentiation Identities}
\begin{align*}
   & \text{\bld{General Differentiation}}                                                        \\
   & \text{Variables}                     & a,~n \in \bb{R},~        & f,~g~\text{is a function} \\
   & \text{Power Rule}                    & \frac{d}{dx} x^n         & = nx^{n-1}                \\
   & \text{Constant}                      & \frac{d}{dx} a           & = 0                       \\
   & \text{Scalar}                        & \frac{d}{dx} af          & = af'                     \\
   & \text{Sum Rule}                      & \frac{d}{dx} f \pm g     & = f' \pm g'               \\
   & \text{Product Rule}                  & \frac{d}{dx}fg           & = fg' + f'g               \\
   & \text{Quotient Rule}                 & \frac{d}{dx} \frac{f}{g} & = \frac{gf'-g'f}{g^2}     \\
\end{align*}
\begin{align*}
  \text{\bld{Trigonometric}} &                  & \text{\bld{Inverse Trigonometric}}                                                       \\
  \frac{d}{dx} \sin x        & = \cos x         & \frac{d}{dx} \sin^{-1} x           & = \frac{1}{\sqrt{1-x^2}}                            \\
  \frac{d}{dx} \cos x        & = -\sin x        & \frac{d}{dx} \cos^{-1} x           & = -\frac{1}{\sqrt{1-x^2}}                           \\
  \frac{d}{dx} \tan x        & = \sec^2 x       & \frac{d}{dx} \tan^{-1} x           & = \frac{1}{1+x^2}                                   \\
  \frac{d}{dx} \cot x        & = -\csc^2 x      & \frac{d}{dx} \cot^{-1} x           & = -\frac{1}{1+x^2}                                  \\
  \frac{d}{dx} \sec x        & = \sec x \tan x  & \frac{d}{dx} \sec^{-1} x           & = \frac{1}{\left\lvert x\right\rvert \sqrt{x^2-1}}  \\
  \frac{d}{dx} \csc x        & = -\csc x \cot x & \frac{d}{dx} \csc^{-1} x           & = -\frac{1}{\left\lvert x\right\rvert \sqrt{x^2-1}}
\end{align*}
\begin{align*}
  \text{\bld{Other Differentiation}}                                                                                     \\
  \frac{d}{dx} a^x      & = a^x \cdot \ln a                                                                              \\
  \frac{d}{dx} e^x      & = e^x                                                                                          \\
  \frac{d}{dx} \log_a x & = \frac{1}{\ln_a x}                                                                            \\
  \frac{d}{dx} \ln x    & = \frac{1}{x}                                                                                  \\
  \frac{dy}{dx}         & = \frac{dy}{du} \times \frac{du}{dx} = \frac{dy}{du} \times \frac{du}{dv} \times \frac{dv}{dx}
\end{align*}